2020/day18/Part1.fst
@@ -1,0 +1,54 @@
+module Part1
+
+open Parser
+open FStar.String
+open FStar.IO
+open FStar.All
+
+(*
+type ast =
+  | Number : n:int -> ast
+  | Add : left:ast -> right:ast -> ast
+  | Mul : left:ast -> right:ast -> ast
+
+*)
+(*
+let parse_number : parser ast =
+  space (parse_apply (fun z -> Number z) unsigned_integer )
+ *)
+
+let rec parse_recursive (input:string) : Tot (parse_result string input) (decreases strlen(input)) =
+    (parse_either_ctx input
+      (parse_forget (literal_char 'x'))
+      (brackets_char input '(' parse_recursive ')'))
+      input
+
+let parse_or_report_fail (x:(parser string)) : ML unit =
+  let line = input_line() in 
+  match x line with
+  | Success tok _ _ -> print_string ("parsed '" ^ tok ^ "'\n" )
+  | ParseError expected at -> print_string( "expecting " ^ expected ^ " at '" ^ at ^ "'\n")
+
+let _ = parse_recursive <: parser string
+  
+let _ = parse_or_report_fail parse_recursive  
+
+(*
+let rec parse_ast (input:string) : Tot (parse_result ast input) (decreases (strlen input)) =
+  parse_either
+    (parse_literal )
+    (brackets "(" parse_ast ")" )
+    input
+  *)
+  
+  (*
+  <|>
+  ( parse_comb 
+     parse_ast 
+     (fun t1 t2 -> (Add t1 t2))
+     (parse_comb
+       (literal "+")
+       (fun op t2 -> t2)       
+       parse_ast ))
+       
+*)
